ocaml/src/CloudantUtil.ml
@@ -38,23 +38,19 @@ let fix_harness harness h =
 
 (* Cloudant stuff *)
 
-let unbox_design_doc design_doc =
-  let db = design_doc.Compiler.cloudant_design_inputdb in
-  let dd = design_doc.Compiler.cloudant_design_doc in
-  (db,dd)
-
 let add_harness harness h s =
   Util.global_replace "%HARNESS%" (fix_harness harness h) s
     
-let add_harness_to_designdoc harness h (db,dd) =
-  let dbname = string_of_char_list db in
-  let designdoc = string_of_char_list dd in
+let add_harness_to_designdoc harness h design_doc =
+  let designdoc = string_of_char_list design_doc.Compiler.cloudant_design_doc in
   let harnessed_designdoc = add_harness harness h designdoc in
-  (char_list_of_string dbname, char_list_of_string harnessed_designdoc)
-
-let stringify_designdoc (db,dd) =
-  let dbname = string_of_char_list db in
-  let designdoc = string_of_char_list dd in
+  { Compiler.cloudant_design_inputdb = design_doc.Compiler.cloudant_design_inputdb;
+    Compiler.cloudant_design_name = design_doc.Compiler.cloudant_design_name;
+    Compiler.cloudant_design_doc = char_list_of_string harnessed_designdoc; }
+    
+let stringify_designdoc design_doc =
+  let dbname = string_of_char_list design_doc.Compiler.cloudant_design_inputdb in
+  let designdoc = string_of_char_list design_doc.Compiler.cloudant_design_doc in
   (dbname, designdoc)
 
 (* Java equivalent: CloudantBackend.makeOneDesign *)
@@ -87,10 +83,7 @@ let add_harness_top harness h (cloudant: QLang.cloudant) : QLang.cloudant =
   let last_expr = cloudant.Compiler.cloudant_final_expr in
   let last_inputs = cloudant.Compiler.cloudant_effective_parameters in
   let harnessed_design_docs =
-    List.map (fun doc -> (add_harness_to_designdoc harness h) (unbox_design_doc doc)) design_docs
-  in
-  let harnessed_design_docs =
-    List.map (fun (x,y) -> { Compiler.cloudant_design_inputdb = x; Compiler.cloudant_design_doc = y; }) harnessed_design_docs
+    List.map (fun doc -> (add_harness_to_designdoc harness h) doc) design_docs
   in
   let harnessed_last_expr =
     add_harness harness h (Util.string_of_char_list last_expr)
@@ -103,5 +96,5 @@ let string_of_cloudant cloudant =
   let design_docs = cloudant.Compiler.cloudant_designs in
   let last_expr = cloudant.Compiler.cloudant_final_expr in
   let last_inputs = cloudant.Compiler.cloudant_effective_parameters in
-  fold_design (List.map (fun doc -> stringify_designdoc (unbox_design_doc doc)) design_docs) (Util.string_of_char_list last_expr) last_inputs
+  fold_design (List.map stringify_designdoc design_docs) (Util.string_of_char_list last_expr) last_inputs
 
