ocaml/src/ParseUtil.ml
@@ -100,6 +100,7 @@ let parse_query l f : (string * QLang.query) =
   | Compiler.L_spark_rdd -> raise (Qcert_Error "No parser for Spark (RDD) available")
   | Compiler.L_spark_df -> raise (Qcert_Error "No parser for Spark (Dataframe) available")
   | Compiler.L_cloudant -> raise (Qcert_Error "No parser for Cloudant available")
+  | Compiler.L_cloudant_whisk -> raise (Qcert_Error "No parser for Cloudant available")
   | Compiler.L_error err ->
       let err = string_of_char_list err in
       raise (Qcert_Error ("No parser for Error language available: "^err))
