ocaml/src/QcertOut.ml
@@ -1,0 +1,51 @@
+(*
+ * Copyright 2015-2017 IBM Corporation
+ *
+ * Licensed under the Apache License, Version 2.0 (the "License");
+ * you may not use this file except in compliance with the License.
+ * You may obtain a copy of the License at
+ *
+ * http://www.apache.org/licenses/LICENSE-2.0
+ *
+ * Unless required by applicable law or agreed to in writing, software
+ * distributed under the License is distributed on an "AS IS" BASIS,
+ * WITHOUT WARRANTIES OR CONDITIONS OF ANY KIND, either express or implied.
+ * See the License for the specific language governing permissions and
+ * limitations under the License.
+ *)
+
+(** This module contains compiler output code *)
+
+open Compiler.EnhancedCompiler
+open PrettyIL
+
+(** Output languages *)
+
+let output_query pconf q =
+  begin match q with
+  | Compiler.Q_camp_rule q -> pretty_query pconf pretty_camp_rule q
+  | Compiler.Q_tech_rule q -> pretty_query pconf pretty_tech_rule q
+  | Compiler.Q_designer_rule q -> pretty_query pconf pretty_designer_rule q
+  | Compiler.Q_camp q -> pretty_query pconf pretty_camp q
+  | Compiler.Q_oql q -> pretty_query pconf pretty_oql q
+  | Compiler.Q_sql q -> pretty_query pconf pretty_sql q
+  | Compiler.Q_sqlpp q -> pretty_query pconf pretty_sqlpp q
+  | Compiler.Q_lambda_nra q -> pretty_query pconf pretty_lambda_nra q
+  | Compiler.Q_nra q -> pretty_query pconf pretty_nra q
+  | Compiler.Q_nraenv_core q -> pretty_query pconf pretty_nraenv_core q
+  | Compiler.Q_nraenv q -> pretty_query pconf pretty_nraenv q
+  | Compiler.Q_nnrc_core q -> pretty_query pconf pretty_nnrc q
+  | Compiler.Q_nnrc q -> pretty_query pconf pretty_nnrc q
+  | Compiler.Q_nnrcmr q -> pretty_query pconf pretty_nnrcmr q
+  | Compiler.Q_cldmr q -> pretty_query pconf pretty_cldmr q
+  | Compiler.Q_dnnrc q -> pretty_query pconf pretty_dnnrc_dataframe q
+  | Compiler.Q_dnnrc_typed q -> pretty_query pconf pretty_dnnrc_dataframe_typed q
+  | Compiler.Q_javascript q -> pretty_query pconf pretty_javascript q
+  | Compiler.Q_java q -> pretty_query pconf pretty_java q
+  | Compiler.Q_spark_rdd q -> pretty_query pconf pretty_spark_rdd q
+  | Compiler.Q_spark_df q -> pretty_query pconf pretty_spark_df q
+  | Compiler.Q_cloudant q -> pretty_query pconf pretty_cloudant q
+  | Compiler.Q_cloudant_whisk q -> pretty_query pconf pretty_cloudant_whisk q
+  | Compiler.Q_error q -> pretty_query pconf pretty_error q
+  end
+
