coq/Compiler/Driver/CompEval.v
@@ -45,6 +45,7 @@ Section CompEval.
   Require Import SparkRDDRuntime.
   Require Import SparkDFRuntime.
   Require Import CloudantRuntime.
+  Require Import CloudantWhiskRuntime.
 
   (* Foreign Support *)
   Require Import ForeignToReduceOps.
@@ -173,6 +174,7 @@ Section CompEval.
       | Q_spark_rdd _ => Ev_out_unsupported ("No evaluation support for "++(name_of_language (language_of_query q)))
       | Q_spark_df _ => Ev_out_unsupported ("No evaluation support for "++(name_of_language (language_of_query q)))
       | Q_cloudant _ => Ev_out_unsupported ("No evaluation support for "++(name_of_language (language_of_query q)))
+      | Q_cloudant_whisk _ => Ev_out_unsupported ("No evaluation support for "++(name_of_language (language_of_query q)))
       | Q_error err => Ev_out_unsupported ("No evaluation support for "++(name_of_language (language_of_query q)))
       end.
 
@@ -200,6 +202,7 @@ Section CompEval.
       | Q_spark_rdd _ => Ev_out_unsupported ("No debug evaluation support for "++(name_of_language (language_of_query q)))
       | Q_spark_df _ => Ev_out_unsupported ("No debug evaluation support for "++(name_of_language (language_of_query q)))
       | Q_cloudant _ => Ev_out_unsupported ("No debug evaluation support for "++(name_of_language (language_of_query q)))
+      | Q_cloudant_whisk _ => Ev_out_unsupported ("No debug evaluation support for "++(name_of_language (language_of_query q)))
       | Q_error err => Ev_out_unsupported ("No debug evaluation support for "++(name_of_language (language_of_query q)))
       end.
 
