coq/Compiler/Driver/CompStat.v
@@ -45,6 +45,7 @@ Section CompStat.
   Require Import SparkRDDRuntime.
   Require Import SparkDFRuntime.
   Require Import CloudantRuntime.
+  Require Import CloudantWhiskRuntime.
 
   Require Import CompilerRuntime.
   Require Import BasicSystem.
@@ -77,6 +78,11 @@ Section CompStat.
   Definition stat_error (q: string) : data :=
     drec
       (("error_stat", dstring "no stat available")
+         :: nil).
+
+  Definition stat_cloudant_whisk (q: cloudant_whisk) : data :=
+    drec
+      (("cloudant_whisk_stat", dstring "no stat available")
          :: nil).
 
   Definition stat_cloudant (q: cloudant) : data :=
@@ -199,6 +205,11 @@ Section CompStat.
   Definition stat_tree_error (q: string) : data :=
     drec
       (("error", stat_error q)
+         :: nil).
+
+  Definition stat_tree_cloudant_whisk (q: cloudant_whisk) : data :=
+    drec
+      (("cloudant_whisk", stat_cloudant_whisk q)
          :: nil).
 
   Definition stat_tree_cloudant (q: cloudant) : data :=
@@ -428,6 +439,7 @@ Section CompStat.
         | Q_spark_rdd q => stat_spark_rdd q
         | Q_spark_df q => stat_spark_df q
         | Q_cloudant q => stat_cloudant q
+        | Q_cloudant_whisk q => stat_cloudant_whisk q
         | Q_error q => stat_error q
         end
     in
@@ -458,6 +470,7 @@ Section CompStat.
         | Q_spark_rdd q => stat_tree_spark_rdd q
         | Q_spark_df q => stat_tree_spark_df q
         | Q_cloudant q => stat_tree_cloudant q
+        | Q_cloudant_whisk q => stat_tree_cloudant_whisk q
         | Q_error q => stat_tree_error q
         end
     in
