coq/Translation/CloudanttoCloudantWhisk.v
@@ -1,0 +1,65 @@
+(*
+ * Copyright 2015-2016 IBM Corporation
+ *
+ * Licensed under the Apache License, Version 2.0 (the "License");
+ * you may not use this file except in compliance with the License.
+ * You may obtain a copy of the License at
+ *
+ * http://www.apache.org/licenses/LICENSE-2.0
+ *
+ * Unless required by applicable law or agreed to in writing, software
+ * distributed under the License is distributed on an "AS IS" BASIS,
+ * WITHOUT WARRANTIES OR CONDITIONS OF ANY KIND, either express or implied.
+ * See the License for the specific language governing permissions and
+ * limitations under the License.
+ *)
+
+Require Import List.
+Require Import String.
+Require Import Utils.
+Require Import BasicRuntime.
+Require Import ForeignToJavaScript.
+Require Import ForeignCloudant.
+Require Import CloudantRuntime.
+Require Import CloudantWhiskRuntime.
+
+Local Open Scope string_scope.
+
+Section CloudanttoCloudantWhisk.
+
+  Context {fruntime:foreign_runtime}.
+  Context {ftojavascript:foreign_to_javascript}.
+  Context {fcloudant:foreign_cloudant}.
+
+  Definition cloudant_design_to_view_action
+             (action_name:string)
+             (design:cloudant_design) : whisk_action :=
+    let design_inputdb := cloudant_design_inputdb design in
+    let design_name := cloudant_design_name design in
+    let design_doc := cloudant_design_doc design in
+    let action_name := action_name ++ "_view_" ++ design_name in
+    (action_name,"// VIEW ACTION TO BE DONE").
+  
+  Definition cloudant_design_to_compute_action
+             (action_name:string)
+             (final_expr:string)
+             (effective_parameters:list string) : whisk_action :=
+    let action_name := action_name ++ "_compute" in
+    (action_name,"// COMPUTE ACTION TO BE DONE").
+
+ 
+  Definition cloudant_to_cloudant_whisk (action_name:string) (q:cloudant) : cloudant_whisk :=
+    (cloudant_design_to_compute_action
+       action_name
+       (cloudant_final_expr q)
+       (cloudant_effective_parameters q))
+      :: (map (cloudant_design_to_view_action action_name)
+              (cloudant_designs q)).
+
+End CloudanttoCloudantWhisk.
+
+(* 
+*** Local Variables: ***
+*** coq-load-path: (("../../coq" "Qcert")) ***
+*** End: ***
+*)
